{
 "cells": [
  {
   "cell_type": "markdown",
   "metadata": {},
   "source": [
    "# <center>PHYS 325 SPRING 2021</center> #\n",
    "## <center>HW 2 </center>##\n",
    "### <center>ANANAY SETHI </center>###"
   ]
  },
  {
   "cell_type": "markdown",
   "metadata": {},
   "source": [
    "**Q.1**\n",
    "\n",
    "Given:\n",
    "$$\\vec{B} = B_o \\hat{y}$$\n",
    "$$\\vec{g} = -g \\hat{z}$$\n",
    "\n",
    "We can define the velocity of the object along the three components of motion as well:\n",
    "$$\\vec{v} = \\left<v_x, v_y, v_z\\right>$$\n",
    "\n",
    "We also know that the object is placed at rest at the origin, at $t = 0$. \n",
    "\n",
    "Using the formula for the magnetic force:\n",
    "\n",
    "$$\\vec{F_B} = q \\left(\\vec{v}\\: \\times\\: \\vec{B}\\right) = \\begin{vmatrix} \\hat{x} & \\hat{y} & \\hat{z} \\\\ v_x & v_y & v_z \\\\ 0 & B_o & 0 \\end{vmatrix}$$\n",
    "\n",
    "$$\\vec{F_B} = q \\left[-v_z B_o \\hat{x} + v_x B_o \\hat{z}\\right]$$\n",
    "\n",
    "Creating our Equations of Motion with the given information:\n",
    "\n",
    "$m\\dot{v_y} = 0$\n",
    "\n",
    "$m\\dot{v_x} = - q v_z B_o$\n",
    "\n",
    "$m\\dot{v_z} = q v_x B_o - m g$\n",
    "\n",
    "Simplifying, we get:\n",
    "\n",
    "$$\\dot{v_x} = - \\frac{q B_o}{m} v_z$$\n",
    "\n",
    "$$\\dot{v_z} =  \\frac{q B_o}{m} v_x - g$$\n",
    "\n",
    "Let us define a constant $k = -\\frac{q B_o}{m}$ to get $\\dot{v_x} = k v_z$ and $\\dot{v_z} = -k \\left(-v_x + \\frac{g}{k}\\right)$. \n",
    "\n",
    "We also define a complex number $\\eta (t) = v_z + i (-v_x + g/k)$. \n",
    "\n",
    "Since $g$ and $k$ are constants, when we differentiate $\\eta(t)$ with respect to $t$:\n",
    "\n",
    "$$\\dot{\\eta}(t) = \\dot{v_z} + i \\left(-\\dot{v_x} + \\dot{(g/k)}\\right) = \\dot{v_z} - i \\dot{v_x}$$\n",
    "$$= -k \\left(-v_x + g/k\\right) - i k v_z$$\n",
    "$$= -k \\left[\\left(-v_x + g/k\\right) - i v_z\\right]$$\n",
    "\n",
    "Using the complex property that $a + ib = - (b + ai)$, we can simplify the equation above to:\n",
    "\n",
    "$$\\dot{\\eta}(t) = -i k \\eta(t)$$\n",
    "\n",
    "Using the method of Separation of Variables:\n",
    "\n",
    "$$\\int\\frac{1}{\\eta} d\\eta = \\int -ik\\: dt$$\n",
    "\n",
    "$$\\ln{\\eta} - \\ln{C} = -ikt$$\n",
    "\n",
    "Where $C$ is a constant of integration we decided to take on the left hand side. This gives us an equation for $\\eta(t)$:\n",
    "\n",
    "$$\\eta(t) = C e^{-ikt}$$\n",
    "\n",
    "To solve for this constant of integration, we need to first identify the equation we have, and then make an educated guess. Let us guess that $C = ce^{i\\delta}$. We then get:\n",
    "\n",
    "$$\\eta(t) = c e^{-ikt + i\\delta} = c e^{-i\\left(kt - \\delta \\right)}$$\n",
    "\n",
    "Using Euler's Expansion, we get:\n",
    "\n",
    "$$\\eta(t) = c \\cos{\\left(kt - \\delta\\right)} - i\\: c \\sin{\\left(kt - \\delta\\right)}$$\n",
    "\n",
    "We now have a real and an imaginary component that we can compare our initial values to. \n",
    "\n",
    "$$v_z = c \\cos{\\left(kt - \\delta\\right)}$$\n",
    "\n",
    "$$\\left(-v_x + g/k\\right) = - c \\sin{\\left(kt - \\delta\\right)}$$\n",
    "\n",
    "We integrate both equations with repect to $t$ to find $x(t)$ and $z(t)$:\n",
    "\n",
    "$$x(t) = \\int c \\sin{\\left(kt - \\delta\\right)} dt + \\int g/k\\: dt = \\frac{-c}{k} \\cos{\\left(kt - \\delta\\right)} + \\frac{gt}{k} + c_x$$\n",
    "\n",
    "$$z(t) = \\int c \\cos{\\left(kt - \\delta\\right)} dt = \\frac{c}{k} \\sin{\\left(kt - \\delta\\right)} + c_z$$\n",
    "\n",
    "We are given initial conditions that the object is at rest at the origin at $t = 0$. This tells us that at $t = 0$, $v_y = 0, c_x = c_y = c_z = 0$. \n",
    "\n",
    "Summarizing the data we have:\n",
    "\n",
    "$$\\boxed{x(t) = \\frac{-c}{k} \\cos{\\left(kt - \\delta\\right)} + \\frac{gt}{k}}$$\n",
    "\n",
    "$$\\boxed{y(t) = 0}$$\n",
    "\n",
    "$$\\boxed{z(t) = \\frac{c}{k} \\sin{\\left(kt - \\delta\\right)}}$$\n",
    "\n",
    "Where $k = \\frac{q B_o}{m}$ is the angular frequency of a \"cycloid\"."
   ]
  },
  {
   "cell_type": "markdown",
   "metadata": {},
   "source": [
    "**Q.2**\n",
    "\n",
    "We will be using cylindrical coordinates to set this problem up. We also must define some variables that we will be using in this setup.\n",
    "$r = l \\sin{\\theta}$, where $r$ is the radius of the circle traced by the tetherball when in uniform circular motion. $l$ is the length of the string of the tetherball, and $\\theta$ is the angle subtended by the tetherball with respect to the vertical. \n",
    "\n",
    "The ball has two forces acting on it - the gravitational acceleration downward, and the tension of the string toward the point of tethering. In coordintes, the force equation can be described as:\n",
    "\n",
    "$$F_{ball} = m\\vec{a} = -T \\sin{\\theta}\\: \\hat{r} + T \\cos{\\theta}\\: \\hat{z} - mg \\hat{z}$$\n",
    "\n",
    "The acceleration for an object in cylindrical coordinates is given by:\n",
    "\n",
    "$$\\vec{a} = \\left(\\ddot{r} - r\\dot{\\phi}^2\\right) \\hat{r} + \\left(r \\ddot{\\phi} + 2\\dot{r}\\dot{\\phi}\\right) \\hat{\\phi} + \\left(\\ddot{z}\\right) \\hat{z}$$\n",
    "\n",
    "Comparing the two equations:\n",
    "\n",
    "$m \\left(\\ddot{r} - r\\dot{\\phi}^2\\right) = - T \\sin{\\theta}$\n",
    "\n",
    "$m \\left(r \\ddot{\\phi} + 2\\dot{r}\\dot{\\phi}\\right) = 0$\n",
    "\n",
    "$m \\ddot{z} = T \\cos{\\theta} - mg$\n",
    "\n",
    "Since $\\theta$ is the vertical angle, and it must remain constant, $\\ddot{r} = \\dot{r} = 0$. Since $z = l \\cos{\\theta}$ is a constant, that means that $\\ddot{z} = \\dot{z} = 0$. This simplifies our equations to be:\n",
    "\n",
    "$T \\cos{\\theta} = mg \\rightarrow T = \\frac{mg}{\\cos{\\theta}}$\n",
    "\n",
    "$m r \\dot{\\phi}^2 = T \\sin{\\theta}$\n",
    "\n",
    "$m r \\ddot{\\phi} = 0$\n",
    "\n",
    "Combining the first and second equations:\n",
    "\n",
    "$$m r \\dot{\\phi}^2 = \\frac{mg}{\\cos{\\theta}} \\sin{\\theta} = m \\left(l \\sin{\\theta}\\right) \\dot{\\phi}^2 \\rightarrow \\dot{\\phi} = \\sqrt{\\frac{g}{l \\cos{\\theta}}}$$\n",
    "\n",
    "**2.(i)**\n",
    "\n",
    "$$\\theta = \\cos^{-1}{\\left(\\frac{mg}{T}\\right)} = \\cos^{-1}{\\left(\\frac{g}{l \\dot{\\phi}^2}\\right)} = \\sin^{-1}{\\left(\\frac{T}{l}\\right)}$$ \n",
    "\n",
    "**2.(ii)**\n",
    "\n",
    "$$\\dot{\\phi} = \\sqrt{\\frac{g}{l \\cos{\\theta}}}$$\n",
    "\n",
    "As $\\dot{\\phi} \\rightarrow 0, \\theta \\rightarrow 0$ such that $\\dot{\\phi} = \\sqrt{\\frac{g}{l \\cos{\\theta}}} \\approx \\sqrt{\\frac{g}{l}}$. \n",
    "\n",
    "The frequency is similar to that of a pendulum, however with different constants."
   ]
  },
  {
   "cell_type": "markdown",
   "metadata": {},
   "source": [
    "**Q.3**\n",
    "\n",
    "At the moment the ball leaves the sphere, we define the following variables:\n",
    "$h$ is the height from the center of the sphere. $R - h$ is the distance from the top of the sphere to the point of leaving. \n",
    "$\\theta$ is the angle subtended from the vertical axis. $v_o$ is the initial horizontal velocity. $N$ is the normal force on the object.\n",
    "\n",
    "Since the gravitational force only acts along the z-axis, the component of the gravitational force along the ball in the $\\hat{r}$ direction is $mg \\cos{\\theta}$.\n",
    "\n",
    "So the force along the $\\hat{r}$ direction is:\n",
    "\n",
    "$$mg \\cos{\\theta} - N = \\frac{m v^2}{R} \\tag{1}$$\n",
    "\n",
    "Where $v \\neq v_o$. \n",
    "\n",
    "Using the Conservation of Energy: $1/2 m v^2 - mgh = 0$, we get an equation in terms of $R$:\n",
    "\n",
    "$$\\frac{1}{2}m v^2 - m g \\left(R - R \\cos{\\theta}\\right) = 0$$\n",
    "\n",
    "$$g R \\left(1 - \\cos{\\theta}\\right) = \\frac{1}{2}\\left(v^2 - {v_o}^2\\right) \\tag{2}$$\n",
    "\n",
    "Putting eqs (1) and (2) together, and the fact that $N = 0$ at the point the ball leaves to solve for $h = R - R \\cos{\\theta}$:\n",
    "\n",
    "$$2 g \\left(R - R\\cos{\\theta}\\right) = g R \\cos{\\theta} - {v_o}^2$$\n",
    "\n",
    "$$\\cos{\\theta} = \\frac{{v_o}^2}{gR} + 2 - 2 \\cos{\\theta}$$\n",
    "\n",
    "$$3 \\cos{\\theta} = 2 + \\frac{{v_o}^2}{gR}$$\n",
    "\n",
    "$$\\cos{\\theta} = \\frac{2}{3} + \\frac{{v_o}^2}{3gR}$$\n",
    "\n",
    "$$h = R - R \\cos{\\theta} = R \\left[1 - \\frac{2}{3} - \\frac{{v_o}^2}{3gR}\\right]$$\n",
    "\n",
    "$$\\boxed{h = \\frac{R}{3}\\left[1 - \\frac{{v_o}^2}{gR}\\right]}$$\n",
    "\n",
    "The angle at which the object loses contact:\n",
    "\n",
    "$$\\boxed{\\theta = \\cos^{-1}{\\left(\\frac{2}{3} + \\frac{{v_o}^2}{3gR}\\right)}}$$\n",
    "\n",
    "This angle depends on the value of $v_o$. If $v_o$ is infinitesimal, then $\\theta$ can be approximated to about $48.19^\\circ$ from the vertical axis. "
   ]
  },
  {
   "cell_type": "markdown",
   "metadata": {},
   "source": [
    "**Q.4**\n",
    "\n",
    "$$\\vec{F_D} = -c |\\vec{v}|\\vec{v} = -cv^2 \\hat{v}$$\n",
    "\n",
    "Here, $\\hat{v} = \\hat{z}$. So the total force acting on the ball is:\n",
    "\n",
    "$$\\vec{F} = m\\vec{a} = -mg\\hat{z} - cv^2\\hat{z}$$\n",
    "\n",
    "$$m\\frac{dv}{dt} = mg - cv^2$$\n",
    "\n",
    "Using the Method of Separation of Variables:\n",
    "\n",
    "$$\\int\\frac{m}{mg - cv^2}dv = \\int dt$$\n",
    "\n",
    "Tried solving this integral using Python Package Sympy, however, the result produced was not in its most simplified state. Therefore, the result for this integral comes from WolframAlpha:\n",
    "\n",
    "$$\\sqrt{\\frac{m}{cg}} \\tanh^{-1}{\\left(v \\sqrt{\\frac{c}{mg}}\\right)} = t$$\n",
    "\n",
    "Bringing this function in terms of $v(t)$:\n",
    "\n",
    "$$\\boxed{v(t) = \\sqrt{\\frac{mg}{c}} \\tanh{\\left(t \\sqrt{\\frac{gc}{m}}\\right)}}$$\n",
    "\n",
    "Now, finding the terminal velocity - \n",
    "\n",
    "$v_{terminal} = CONSTANT$, which means $\\frac{dv}{dt}|_{v = v_T} = 0$. This tells us that \n",
    "\n",
    "$$mg - cv^2 = 0 \\rightarrow mg = cv^2 \\rightarrow \\boxed{v_T = \\sqrt{\\frac{mg}{c}}}$$\n",
    "\n",
    "This can also come from the previous result when we assume that $\\tanh{\\left(t \\sqrt{\\frac{gc}{m}}\\right)} \\rightarrow 1$."
   ]
  }
 ],
 "metadata": {
  "kernelspec": {
   "display_name": "Python 3",
   "language": "python",
   "name": "python3"
  },
  "language_info": {
   "codemirror_mode": {
    "name": "ipython",
    "version": 3
   },
   "file_extension": ".py",
   "mimetype": "text/x-python",
   "name": "python",
   "nbconvert_exporter": "python",
   "pygments_lexer": "ipython3",
   "version": "3.8.3"
  }
 },
 "nbformat": 4,
 "nbformat_minor": 2
}
